examples/incr_cas/IncrementIAproof.v
@@ -1,0 +1,77 @@
+Require Import CRIS.
+Require Import SchHeader SchA SchTactics.
+Require Import ImpPrelude MemHeader MemA MemTactics.
+Require Import IncrementHeader IncrementI IncrementA.
+
+Module IncrementIA. Section IncrementIA.
+  Context `{!crisG Γ Σ α β τ _S _I, !memG, !concG, !newschG}.
+
+  Local Definition IstFull := (IstProd (IstSB IncrementA.t.(Mod.scopes) IstTrue) IstEq).
+  Local Definition MA := (IncrementA.t ★ (MemA.t sp_none)).
+  Local Definition MI := (IncrementI.t ★ (MemA.t sp_none)).
+
+  Lemma increment_simF : ISim.sim_fun open MA MI True%I IstFull (Some IncrementHdr.increment).
+  Proof.
+    init_simF.
+    steps_l. destruct _q; ss. destruct _q; ss. destruct v; ss. inv G0. hss.
+    destruct _q0 as [blk ofs].
+
+    steps_r.
+    sch_yield_rr.
+    steps_r. sch_yield_rr.
+    sch_yield_l.
+    norm_l. norm_r.
+
+    iApply wsim_reset.
+    iStopProof. revert st_src. combine_quant st_tgt.
+    eapply wsim_coind.
+    iIntros (g' _ CIH [st_t st_s]) "%GG' /=".
+    destruct_quant CIH.
+
+    unfold_iterC_l. unfold_iterC_r.
+    steps_l. steps_r.
+    sch_yield_rr.
+    Unshelve. all: try exact 0.
+
+    sch_yield_l. steps_l. rename _q into v.
+
+    steps_r. inline_r. force_r (blk, ofs, 1%Qp, Vint v). steps_r.
+    forces_r. iFrame "ASM". iSplit; eauto.
+    steps_r. iDestruct "GRT" as "[[PT ->] ->]". hss_r. steps_r.
+
+    force_l false. steps_l. force_l; iFrame "PT". steps_l. sch_yield_l. steps_l.
+    unfold_iterC_l. steps_l.
+
+    sch_yield_rr. steps_r.
+    sch_yield_rr. steps_r.
+
+    sch_yield_l. steps_l. rename _q into v'.
+    iApply (wsim_mem_cas _ _ _ _ _ _ _ _ _ _ _ _ _ _ _ _ _ emp%I with "ASM");
+        [try prove_inline_cond|try prove_sb_cond|unfold_cris_defs|..]; eauto.
+    { des_ifs. }
+    { iIntros "_"; iExists _, _, _, _; ss. }
+    iIntros "H _".
+    Unshelve. all: try exact 0; try exact 1%Qp; try exact (Vint 0).
+
+    steps_r. hss_r. steps_r.
+    destruct (dec v' v) as [?|Heq]; [subst; ss|ss].
+    { force_l true. steps_l. force_l; iFrame "H"; steps_l.
+      sch_yield_rr. steps_r.
+      sch_yield_rr; steps_r.
+      case_decide; [|ss].
+      steps_r.
+      sch_yield_l. steps_l. step. iSplit; done.
+    }
+    { force_l false.
+      forces_l. iFrame "H". steps_l.
+      sch_yield_rr; steps_r.
+      sch_yield_rr; steps_r.
+      case_decide; first clarify.
+      steps_r.
+      sch_yield_l. steps_l.
+      iApply wsim_progress. iApply wsim_base.
+      iIntros "?". iApply (CIH). iFrame.
+    }
+    Unshelve. all: eauto.
+  (*SLOW*)Qed.
+End IncrementIA. End IncrementIA.
