examples/incr_faa/FaaI.v
@@ -1,0 +1,28 @@
+Require Import CRIS.
+Require Import ImpPrelude MemHeader MemA SchA SchTactics SchHeader.
+Require Import FaaHeader.
+
+Module FaaI. Section FaaI.
+  Context `{!crisG Γ Σ α β τ _S _I, !concG}.
+
+  Definition scopes : list string := [].
+
+  Definition faa2 : list val → itree crisE unit :=
+    λ arg,
+      𝒴;;; '_ : val <- MemHdr.faa arg;;
+      𝒴;;; '_ : val <- MemHdr.faa arg;;
+      𝒴;;; Ret tt.
+
+  Definition fnsems : fnsems_type :=
+    [(Some FaaHdr.faa2, (false, wmask_all, scopes, (None, cfunU faa2)))].
+
+  Program Definition smod : SMod.t := {|
+    SMod.scopes := scopes;
+    SMod.fnsems := fnsems;
+    SMod.initial_st := [];
+  |}.
+  Solve All Obligations with prove_scope.
+  Next Obligation. prove_nodup. Qed.
+
+  Definition t : Mod.t := Seal.sealing CRIS (SMod.to_mod sp_none smod).
+End FaaI. End FaaI.
